Back to normal order semanics; proved strong normalization with errors

src/Log.v
@@ -42,10 +42,10 @@ Variable R : ∀ {τ}, Exp Γ τ → Exp Γ τ → Prop.
     expressions. *)
 Equations ExpR {τ} (e1 e2 : Exp Γ τ) : Prop :=
   ExpR (τ:=_ ⟶ _) f1 f2 :=
-    R f1 f2 ∧ (∀ x1 x2, ExpR x1 x2 → ExpR (APP f1 x1) (APP f1 x1));
+    R f1 f2 ∧ (∀ x1 x2, ExpR x1 x2 → ExpR (APP f1 x1) (APP f1 x2));
   ExpR e1 e2 := R e1 e2.
 
-Lemma ExpR_P {τ} {e1 e2 : Γ ⊢ τ} : ExpR e1 e2 → R e1 e2.
+Lemma ExpR_R {τ} {e1 e2 : Γ ⊢ τ} : ExpR e1 e2 → R e1 e2.
 Proof. intros; induction τ; simpl in *; simp ExpR in H; now reduce. Qed.
 
 End Log.
